<script lang="ts">
	import { noteInfo } from '$lib/note/note';
	noteInfo('Topic List', '/');
</script>
# Hello World

The quadratic equation $ax^2+bx+c=0$ has roots

$$
x = \frac{-b \pm \sqrt{b^2-4ac}}{2a}
$$
$$
x = \frac{-b \pm \sqrt{b^2-4ac}}{2a}
$$
$$
x = \frac{-b \pm \sqrt{b^2-4ac}}{2a}
$$
$$
x = \frac{-b \pm \sqrt{b^2-4ac}}{2a}
$$
$$
x = \frac{-b \pm \sqrt{b^2-4ac}}{2a}
$$
$$
x = \frac{-b \pm \sqrt{b^2-4ac}}{2a}
$$
$$
x = \frac{-b \pm \sqrt{b^2-4ac}}{2a}
$$
$$
x = \frac{-b \pm \sqrt{b^2-4ac}}{2a}
$$
$$
x = \frac{-b \pm \sqrt{b^2-4ac}}{2a}
$$
$$
x = \frac{-b \pm \sqrt{b^2-4ac}}{2a}
$$
$$
x = \frac{-b \pm \sqrt{b^2-4ac}}{2a}
$$
$$
x = \frac{-b \pm \sqrt{b^2-4ac}}{2a}
$$
$$
x = \frac{-b \pm \sqrt{b^2-4ac}}{2a}
$$
$$
x = \frac{-b \pm \sqrt{b^2-4ac}}{2a}
$$
$$
x = \frac{-b \pm \sqrt{b^2-4ac}}{2a}
$$
$$
x = \frac{-b \pm \sqrt{b^2-4ac}}{2a}
$$
$$
x = \frac{-b \pm \sqrt{b^2-4ac}}{2a}
$$
$$
x = \frac{-b \pm \sqrt{b^2-4ac}}{2a}
$$
$$
x = \frac{-b \pm \sqrt{b^2-4ac}}{2a}
$$
$$
x = \frac{-b \pm \sqrt{b^2-4ac}}{2a}
$$
$$
x = \frac{-b \pm \sqrt{b^2-4ac}}{2a}
$$
$$
x = \frac{-b \pm \sqrt{b^2-4ac}}{2a}
$$
$$
x = \frac{-b \pm \sqrt{b^2-4ac}}{2a}
$$
$$
x = \frac{-b \pm \sqrt{b^2-4ac}}{2a}
$$
$$
x = \frac{-b \pm \sqrt{b^2-4ac}}{2a}
$$
$$
x = \frac{-b \pm \sqrt{b^2-4ac}}{2a}
$$
$$
x = \frac{-b \pm \sqrt{b^2-4ac}}{2a}
$$
$$
x = \frac{-b \pm \sqrt{b^2-4ac}}{2a}
$$
$$
x = \frac{-b \pm \sqrt{b^2-4ac}}{2a}
$$
$$
x = \frac{-b \pm \sqrt{b^2-4ac}}{2a}
$$
$$
x = \frac{-b \pm \sqrt{b^2-4ac}}{2a}
$$
$$
x = \frac{-b \pm \sqrt{b^2-4ac}}{2a}
$$
$$
x = \frac{-b \pm \sqrt{b^2-4ac}}{2a}
$$
$$
x = \frac{-b \pm \sqrt{b^2-4ac}}{2a}
$$
$$
x = \frac{-b \pm \sqrt{b^2-4ac}}{2a}
$$
$$
x = \frac{-b \pm \sqrt{b^2-4ac}}{2a}
$$
$$
x = \frac{-b \pm \sqrt{b^2-4ac}}{2a}
$$
$$
x = \frac{-b \pm \sqrt{b^2-4ac}}{2a}
$$
$$
x = \frac{-b \pm \sqrt{b^2-4ac}}{2a}
$$
$$
x = \frac{-b \pm \sqrt{b^2-4ac}}{2a}
$$
$$
x = \frac{-b \pm \sqrt{b^2-4ac}}{2a}
$$
$$
x = \frac{-b \pm \sqrt{b^2-4ac}}{2a}
$$
$$
x = \frac{-b \pm \sqrt{b^2-4ac}}{2a}
$$
$$
x = \frac{-b \pm \sqrt{b^2-4ac}}{2a}
$$
$$
x = \frac{-b \pm \sqrt{b^2-4ac}}{2a}
$$
$$
x = \frac{-b \pm \sqrt{b^2-4ac}}{2a}
$$
$$
x = \frac{-b \pm \sqrt{b^2-4ac}}{2a}
$$
$$
x = \frac{-b \pm \sqrt{b^2-4ac}}{2a}
$$
$$
x = \frac{-b \pm \sqrt{b^2-4ac}}{2a}
$$
$$
x = \frac{-b \pm \sqrt{b^2-4ac}}{2a}
$$
$$
x = \frac{-b \pm \sqrt{b^2-4ac}}{2a}
$$
$$
x = \frac{-b \pm \sqrt{b^2-4ac}}{2a}
$$
$$
x = \frac{-b \pm \sqrt{b^2-4ac}}{2a}
$$
$$
x = \frac{-b \pm \sqrt{b^2-4ac}}{2a}
$$
$$
x = \frac{-b \pm \sqrt{b^2-4ac}}{2a}
$$
$$
x = \frac{-b \pm \sqrt{b^2-4ac}}{2a}
$$
$$
x = \frac{-b \pm \sqrt{b^2-4ac}}{2a}
$$
$$
x = \frac{-b \pm \sqrt{b^2-4ac}}{2a}
$$
$$
x = \frac{-b \pm \sqrt{b^2-4ac}}{2a}
$$
$$
x = \frac{-b \pm \sqrt{b^2-4ac}}{2a}
$$
$$
x = \frac{-b \pm \sqrt{b^2-4ac}}{2a}
$$
$$
x = \frac{-b \pm \sqrt{b^2-4ac}}{2a}
$$
$$
x = \frac{-b \pm \sqrt{b^2-4ac}}{2a}
$$
$$
x = \frac{-b \pm \sqrt{b^2-4ac}}{2a}
$$
$$
x = \frac{-b \pm \sqrt{b^2-4ac}}{2a}
$$
$$
x = \frac{-b \pm \sqrt{b^2-4ac}}{2a}
$$
$$
x = \frac{-b \pm \sqrt{b^2-4ac}}{2a}
$$
$$
x = \frac{-b \pm \sqrt{b^2-4ac}}{2a}
$$
$$
x = \frac{-b \pm \sqrt{b^2-4ac}}{2a}
$$
